% backtracking worksheet template
\documentclass[leqno, 12pt]{article}
\usepackage{tikz}  
\usetikzlibrary{positioning}
\usetikzlibrary {arrows.meta}
\usepackage[a4paper, portrait, margin=1cm]{geometry}
\usepackage{multicol}
\usepackage{fancyhdr}

\tikzset{backtrack/.style={rectangle,draw=black,fill=white,
inner sep=2pt,minimum height=32pt, minimum width=20mm}}
\tikzset{backtrackeq/.style={rectangle,draw=black,fill=white,
inner sep=2pt,minimum height=12pt, minimum width=20mm}}
\tikzset{backtrackstep/.style={rectangle,draw=none,fill=white,
inner sep=2pt,minimum height=12pt, minimum width=20mm}}

\def \HeadingAnswers {\section*{\Large Name: \underline{\hspace{8cm}} \hfill Date: \underline{\hspace{3cm}}} \vspace{-3mm}
{2-step backtracking: Answers} \vspace{1pt}\hrule}

% raise footer with page number; no header
\fancypagestyle{myfancypagestyle}{
  \fancyhf{}% clear all header and footer fields
  \renewcommand{\headrulewidth}{0pt} % no rule under header
  \fancyfoot[C] {\thepage} \setlength{\footskip}{6pt} % raise page number 6pt
}
\pagestyle{myfancypagestyle}  % apply myfancypagestyle

\begin{document}
    \HeadingAnswers
    \vspace{-8mm}
    \begin{multicols}{2}
        \begin{equation}
    \begin{tikzpicture}[baseline={([yshift=-12pt]current bounding box.north)}]

        \node[backtrack] (boxA) at (0, 0) {$x$};
        \node[backtrack] (boxB) [right=1cm of boxA] {$4x$};
        \node[backtrack] (boxC) [right=1cm of boxB] {$4x - 10$};
    
        \node (boxAr) at ([yshift=24pt,xshift=5mm]boxA) { };
        \node (boxBl) at ([yshift=24pt,xshift=-5mm]boxB) { };
        \draw [line width=0.4pt,-{Stealth[length=2mm]}] (boxAr)  --node[backtrackstep, above=3.0pt] {$\times4$} (boxBl);
    
        \node (boxBr) at ([yshift=24pt,xshift=5mm]boxB) { };
        \node (boxCl) at ([yshift=24pt,xshift=-5mm]boxC) { };
        \draw [line width=0.4pt,-{Stealth[length=2mm]}] (boxBr)  --node[backtrackstep, above=3.0pt] {$-10$} (boxCl);
        
    \end{tikzpicture} 
\end{equation}


\vspace{-2pt}\begin{equation}
    \begin{tikzpicture}[baseline={([yshift=-12pt]current bounding box.north)}]

        \node[backtrack] (boxA) at (0, 0) {$x$};
        \node[backtrack] (boxB) [right=1cm of boxA] {$x-3$};
        \node[backtrack] (boxC) [right=1cm of boxB] {$\frac{(x-3)}{3}$};
    
        \node (boxAr) at ([yshift=24pt,xshift=5mm]boxA) { };
        \node (boxBl) at ([yshift=24pt,xshift=-5mm]boxB) { };
        \draw [line width=0.4pt,-{Stealth[length=2mm]}] (boxAr)  --node[backtrackstep, above=3.0pt] {$-3$} (boxBl);
    
        \node (boxBr) at ([yshift=24pt,xshift=5mm]boxB) { };
        \node (boxCl) at ([yshift=24pt,xshift=-5mm]boxC) { };
        \draw [line width=0.4pt,-{Stealth[length=2mm]}] (boxBr)  --node[backtrackstep, above=3.0pt] {$\div3$} (boxCl);
        
    \end{tikzpicture} 
\end{equation}


\vspace{-2pt}\begin{equation}
    \begin{tikzpicture}[baseline={([yshift=-12pt]current bounding box.north)}]

        \node[backtrack] (boxA) at (0, 0) {$x$};
        \node[backtrack] (boxB) [right=1cm of boxA] {$x+9$};
        \node[backtrack] (boxC) [right=1cm of boxB] {$8(x + 9)$};
    
        \node (boxAr) at ([yshift=24pt,xshift=5mm]boxA) { };
        \node (boxBl) at ([yshift=24pt,xshift=-5mm]boxB) { };
        \draw [line width=0.4pt,-{Stealth[length=2mm]}] (boxAr)  --node[backtrackstep, above=3.0pt] {$+9$} (boxBl);
    
        \node (boxBr) at ([yshift=24pt,xshift=5mm]boxB) { };
        \node (boxCl) at ([yshift=24pt,xshift=-5mm]boxC) { };
        \draw [line width=0.4pt,-{Stealth[length=2mm]}] (boxBr)  --node[backtrackstep, above=3.0pt] {$\times8$} (boxCl);
        
    \end{tikzpicture} 
\end{equation}


\vspace{-2pt}\begin{equation}
    \begin{tikzpicture}[baseline={([yshift=-12pt]current bounding box.north)}]

        \node[backtrack] (boxA) at (0, 0) {$x$};
        \node[backtrack] (boxB) [right=1cm of boxA] {$x-8$};
        \node[backtrack] (boxC) [right=1cm of boxB] {$8(x-8)$};
    
        \node (boxAr) at ([yshift=24pt,xshift=5mm]boxA) { };
        \node (boxBl) at ([yshift=24pt,xshift=-5mm]boxB) { };
        \draw [line width=0.4pt,-{Stealth[length=2mm]}] (boxAr)  --node[backtrackstep, above=3.0pt] {$-8$} (boxBl);
    
        \node (boxBr) at ([yshift=24pt,xshift=5mm]boxB) { };
        \node (boxCl) at ([yshift=24pt,xshift=-5mm]boxC) { };
        \draw [line width=0.4pt,-{Stealth[length=2mm]}] (boxBr)  --node[backtrackstep, above=3.0pt] {$\times8$} (boxCl);
        
    \end{tikzpicture} 
\end{equation}


\vspace{-2pt}\begin{equation}
    \begin{tikzpicture}[baseline={([yshift=-12pt]current bounding box.north)}]

        \node[backtrack] (boxA) at (0, 0) {$x$};
        \node[backtrack] (boxB) [right=1cm of boxA] {$4x$};
        \node[backtrack] (boxC) [right=1cm of boxB] {$4x - 6$};
    
        \node (boxAr) at ([yshift=24pt,xshift=5mm]boxA) { };
        \node (boxBl) at ([yshift=24pt,xshift=-5mm]boxB) { };
        \draw [line width=0.4pt,-{Stealth[length=2mm]}] (boxAr)  --node[backtrackstep, above=3.0pt] {$\times4$} (boxBl);
    
        \node (boxBr) at ([yshift=24pt,xshift=5mm]boxB) { };
        \node (boxCl) at ([yshift=24pt,xshift=-5mm]boxC) { };
        \draw [line width=0.4pt,-{Stealth[length=2mm]}] (boxBr)  --node[backtrackstep, above=3.0pt] {$-6$} (boxCl);
        
    \end{tikzpicture} 
\end{equation}


\vspace{-2pt}\begin{equation}
    \begin{tikzpicture}[baseline={([yshift=-12pt]current bounding box.north)}]

        \node[backtrack] (boxA) at (0, 0) {$x$};
        \node[backtrack] (boxB) [right=1cm of boxA] {$\frac{x}{5}$};
        \node[backtrack] (boxC) [right=1cm of boxB] {$\frac{x}{5} + 3$};
    
        \node (boxAr) at ([yshift=24pt,xshift=5mm]boxA) { };
        \node (boxBl) at ([yshift=24pt,xshift=-5mm]boxB) { };
        \draw [line width=0.4pt,-{Stealth[length=2mm]}] (boxAr)  --node[backtrackstep, above=3.0pt] {$\div5$} (boxBl);
    
        \node (boxBr) at ([yshift=24pt,xshift=5mm]boxB) { };
        \node (boxCl) at ([yshift=24pt,xshift=-5mm]boxC) { };
        \draw [line width=0.4pt,-{Stealth[length=2mm]}] (boxBr)  --node[backtrackstep, above=3.0pt] {$+3$} (boxCl);
        
    \end{tikzpicture} 
\end{equation}


\vspace{-2pt}\begin{equation}
    \begin{tikzpicture}[baseline={([yshift=-12pt]current bounding box.north)}]

        \node[backtrack] (boxA) at (0, 0) {$x$};
        \node[backtrack] (boxB) [right=1cm of boxA] {$3x$};
        \node[backtrack] (boxC) [right=1cm of boxB] {$3x - 3$};
    
        \node (boxAr) at ([yshift=24pt,xshift=5mm]boxA) { };
        \node (boxBl) at ([yshift=24pt,xshift=-5mm]boxB) { };
        \draw [line width=0.4pt,-{Stealth[length=2mm]}] (boxAr)  --node[backtrackstep, above=3.0pt] {$\times3$} (boxBl);
    
        \node (boxBr) at ([yshift=24pt,xshift=5mm]boxB) { };
        \node (boxCl) at ([yshift=24pt,xshift=-5mm]boxC) { };
        \draw [line width=0.4pt,-{Stealth[length=2mm]}] (boxBr)  --node[backtrackstep, above=3.0pt] {$-3$} (boxCl);
        
    \end{tikzpicture} 
\end{equation}


\vspace{-2pt}\begin{equation}
    \begin{tikzpicture}[baseline={([yshift=-12pt]current bounding box.north)}]

        \node[backtrack] (boxA) at (0, 0) {$x$};
        \node[backtrack] (boxB) [right=1cm of boxA] {$9x$};
        \node[backtrack] (boxC) [right=1cm of boxB] {$9x - 10$};
    
        \node (boxAr) at ([yshift=24pt,xshift=5mm]boxA) { };
        \node (boxBl) at ([yshift=24pt,xshift=-5mm]boxB) { };
        \draw [line width=0.4pt,-{Stealth[length=2mm]}] (boxAr)  --node[backtrackstep, above=3.0pt] {$\times9$} (boxBl);
    
        \node (boxBr) at ([yshift=24pt,xshift=5mm]boxB) { };
        \node (boxCl) at ([yshift=24pt,xshift=-5mm]boxC) { };
        \draw [line width=0.4pt,-{Stealth[length=2mm]}] (boxBr)  --node[backtrackstep, above=3.0pt] {$-10$} (boxCl);
        
    \end{tikzpicture} 
\end{equation}


\vspace{-2pt}\begin{equation}
    \begin{tikzpicture}[baseline={([yshift=-12pt]current bounding box.north)}]

        \node[backtrack] (boxA) at (0, 0) {$x$};
        \node[backtrack] (boxB) [right=1cm of boxA] {$x+2$};
        \node[backtrack] (boxC) [right=1cm of boxB] {$\frac{(x+2)}{2}$};
    
        \node (boxAr) at ([yshift=24pt,xshift=5mm]boxA) { };
        \node (boxBl) at ([yshift=24pt,xshift=-5mm]boxB) { };
        \draw [line width=0.4pt,-{Stealth[length=2mm]}] (boxAr)  --node[backtrackstep, above=3.0pt] {$+2$} (boxBl);
    
        \node (boxBr) at ([yshift=24pt,xshift=5mm]boxB) { };
        \node (boxCl) at ([yshift=24pt,xshift=-5mm]boxC) { };
        \draw [line width=0.4pt,-{Stealth[length=2mm]}] (boxBr)  --node[backtrackstep, above=3.0pt] {$\div2$} (boxCl);
        
    \end{tikzpicture} 
\end{equation}


\vspace{-2pt}\begin{equation}
    \begin{tikzpicture}[baseline={([yshift=-12pt]current bounding box.north)}]

        \node[backtrack] (boxA) at (0, 0) {$x$};
        \node[backtrack] (boxB) [right=1cm of boxA] {$10x$};
        \node[backtrack] (boxC) [right=1cm of boxB] {$10x - 2$};
    
        \node (boxAr) at ([yshift=24pt,xshift=5mm]boxA) { };
        \node (boxBl) at ([yshift=24pt,xshift=-5mm]boxB) { };
        \draw [line width=0.4pt,-{Stealth[length=2mm]}] (boxAr)  --node[backtrackstep, above=3.0pt] {$\times10$} (boxBl);
    
        \node (boxBr) at ([yshift=24pt,xshift=5mm]boxB) { };
        \node (boxCl) at ([yshift=24pt,xshift=-5mm]boxC) { };
        \draw [line width=0.4pt,-{Stealth[length=2mm]}] (boxBr)  --node[backtrackstep, above=3.0pt] {$-2$} (boxCl);
        
    \end{tikzpicture} 
\end{equation}


\vspace{-2pt}\begin{equation}
    \begin{tikzpicture}[baseline={([yshift=-12pt]current bounding box.north)}]

        \node[backtrack] (boxA) at (0, 0) {$x$};
        \node[backtrack] (boxB) [right=1cm of boxA] {$x-3$};
        \node[backtrack] (boxC) [right=1cm of boxB] {$\frac{(x-3)}{5}$};
    
        \node (boxAr) at ([yshift=24pt,xshift=5mm]boxA) { };
        \node (boxBl) at ([yshift=24pt,xshift=-5mm]boxB) { };
        \draw [line width=0.4pt,-{Stealth[length=2mm]}] (boxAr)  --node[backtrackstep, above=3.0pt] {$-3$} (boxBl);
    
        \node (boxBr) at ([yshift=24pt,xshift=5mm]boxB) { };
        \node (boxCl) at ([yshift=24pt,xshift=-5mm]boxC) { };
        \draw [line width=0.4pt,-{Stealth[length=2mm]}] (boxBr)  --node[backtrackstep, above=3.0pt] {$\div5$} (boxCl);
        
    \end{tikzpicture} 
\end{equation}


\vspace{-2pt}\begin{equation}
    \begin{tikzpicture}[baseline={([yshift=-12pt]current bounding box.north)}]

        \node[backtrack] (boxA) at (0, 0) {$x$};
        \node[backtrack] (boxB) [right=1cm of boxA] {$\frac{x}{3}$};
        \node[backtrack] (boxC) [right=1cm of boxB] {$\frac{x}{3} + 6$};
    
        \node (boxAr) at ([yshift=24pt,xshift=5mm]boxA) { };
        \node (boxBl) at ([yshift=24pt,xshift=-5mm]boxB) { };
        \draw [line width=0.4pt,-{Stealth[length=2mm]}] (boxAr)  --node[backtrackstep, above=3.0pt] {$\div3$} (boxBl);
    
        \node (boxBr) at ([yshift=24pt,xshift=5mm]boxB) { };
        \node (boxCl) at ([yshift=24pt,xshift=-5mm]boxC) { };
        \draw [line width=0.4pt,-{Stealth[length=2mm]}] (boxBr)  --node[backtrackstep, above=3.0pt] {$+6$} (boxCl);
        
    \end{tikzpicture} 
\end{equation}


\vspace{-2pt}\begin{equation}
    \begin{tikzpicture}[baseline={([yshift=-12pt]current bounding box.north)}]

        \node[backtrack] (boxA) at (0, 0) {$x$};
        \node[backtrack] (boxB) [right=1cm of boxA] {$10x$};
        \node[backtrack] (boxC) [right=1cm of boxB] {$10x + 9$};
    
        \node (boxAr) at ([yshift=24pt,xshift=5mm]boxA) { };
        \node (boxBl) at ([yshift=24pt,xshift=-5mm]boxB) { };
        \draw [line width=0.4pt,-{Stealth[length=2mm]}] (boxAr)  --node[backtrackstep, above=3.0pt] {$\times10$} (boxBl);
    
        \node (boxBr) at ([yshift=24pt,xshift=5mm]boxB) { };
        \node (boxCl) at ([yshift=24pt,xshift=-5mm]boxC) { };
        \draw [line width=0.4pt,-{Stealth[length=2mm]}] (boxBr)  --node[backtrackstep, above=3.0pt] {$+9$} (boxCl);
        
    \end{tikzpicture} 
\end{equation}


\vspace{-2pt}\begin{equation}
    \begin{tikzpicture}[baseline={([yshift=-12pt]current bounding box.north)}]

        \node[backtrack] (boxA) at (0, 0) {$x$};
        \node[backtrack] (boxB) [right=1cm of boxA] {$2x$};
        \node[backtrack] (boxC) [right=1cm of boxB] {$2x + 7$};
    
        \node (boxAr) at ([yshift=24pt,xshift=5mm]boxA) { };
        \node (boxBl) at ([yshift=24pt,xshift=-5mm]boxB) { };
        \draw [line width=0.4pt,-{Stealth[length=2mm]}] (boxAr)  --node[backtrackstep, above=3.0pt] {$\times2$} (boxBl);
    
        \node (boxBr) at ([yshift=24pt,xshift=5mm]boxB) { };
        \node (boxCl) at ([yshift=24pt,xshift=-5mm]boxC) { };
        \draw [line width=0.4pt,-{Stealth[length=2mm]}] (boxBr)  --node[backtrackstep, above=3.0pt] {$+7$} (boxCl);
        
    \end{tikzpicture} 
\end{equation}


\vspace{-2pt}\begin{equation}
    \begin{tikzpicture}[baseline={([yshift=-12pt]current bounding box.north)}]

        \node[backtrack] (boxA) at (0, 0) {$x$};
        \node[backtrack] (boxB) [right=1cm of boxA] {$\frac{x}{3}$};
        \node[backtrack] (boxC) [right=1cm of boxB] {$\frac{x}{3} + 5$};
    
        \node (boxAr) at ([yshift=24pt,xshift=5mm]boxA) { };
        \node (boxBl) at ([yshift=24pt,xshift=-5mm]boxB) { };
        \draw [line width=0.4pt,-{Stealth[length=2mm]}] (boxAr)  --node[backtrackstep, above=3.0pt] {$\div3$} (boxBl);
    
        \node (boxBr) at ([yshift=24pt,xshift=5mm]boxB) { };
        \node (boxCl) at ([yshift=24pt,xshift=-5mm]boxC) { };
        \draw [line width=0.4pt,-{Stealth[length=2mm]}] (boxBr)  --node[backtrackstep, above=3.0pt] {$+5$} (boxCl);
        
    \end{tikzpicture} 
\end{equation}


\vspace{-2pt}\begin{equation}
    \begin{tikzpicture}[baseline={([yshift=-12pt]current bounding box.north)}]

        \node[backtrack] (boxA) at (0, 0) {$x$};
        \node[backtrack] (boxB) [right=1cm of boxA] {$x-4$};
        \node[backtrack] (boxC) [right=1cm of boxB] {$8(x-4)$};
    
        \node (boxAr) at ([yshift=24pt,xshift=5mm]boxA) { };
        \node (boxBl) at ([yshift=24pt,xshift=-5mm]boxB) { };
        \draw [line width=0.4pt,-{Stealth[length=2mm]}] (boxAr)  --node[backtrackstep, above=3.0pt] {$-4$} (boxBl);
    
        \node (boxBr) at ([yshift=24pt,xshift=5mm]boxB) { };
        \node (boxCl) at ([yshift=24pt,xshift=-5mm]boxC) { };
        \draw [line width=0.4pt,-{Stealth[length=2mm]}] (boxBr)  --node[backtrackstep, above=3.0pt] {$\times8$} (boxCl);
        
    \end{tikzpicture} 
\end{equation}


\vspace{-2pt}\begin{equation}
    \begin{tikzpicture}[baseline={([yshift=-12pt]current bounding box.north)}]

        \node[backtrack] (boxA) at (0, 0) {$x$};
        \node[backtrack] (boxB) [right=1cm of boxA] {$x-4$};
        \node[backtrack] (boxC) [right=1cm of boxB] {$2(x-4)$};
    
        \node (boxAr) at ([yshift=24pt,xshift=5mm]boxA) { };
        \node (boxBl) at ([yshift=24pt,xshift=-5mm]boxB) { };
        \draw [line width=0.4pt,-{Stealth[length=2mm]}] (boxAr)  --node[backtrackstep, above=3.0pt] {$-4$} (boxBl);
    
        \node (boxBr) at ([yshift=24pt,xshift=5mm]boxB) { };
        \node (boxCl) at ([yshift=24pt,xshift=-5mm]boxC) { };
        \draw [line width=0.4pt,-{Stealth[length=2mm]}] (boxBr)  --node[backtrackstep, above=3.0pt] {$\times2$} (boxCl);
        
    \end{tikzpicture} 
\end{equation}


\vspace{-2pt}\begin{equation}
    \begin{tikzpicture}[baseline={([yshift=-12pt]current bounding box.north)}]

        \node[backtrack] (boxA) at (0, 0) {$x$};
        \node[backtrack] (boxB) [right=1cm of boxA] {$x+1$};
        \node[backtrack] (boxC) [right=1cm of boxB] {$\frac{(x+1)}{1}$};
    
        \node (boxAr) at ([yshift=24pt,xshift=5mm]boxA) { };
        \node (boxBl) at ([yshift=24pt,xshift=-5mm]boxB) { };
        \draw [line width=0.4pt,-{Stealth[length=2mm]}] (boxAr)  --node[backtrackstep, above=3.0pt] {$+1$} (boxBl);
    
        \node (boxBr) at ([yshift=24pt,xshift=5mm]boxB) { };
        \node (boxCl) at ([yshift=24pt,xshift=-5mm]boxC) { };
        \draw [line width=0.4pt,-{Stealth[length=2mm]}] (boxBr)  --node[backtrackstep, above=3.0pt] {$\div1$} (boxCl);
        
    \end{tikzpicture} 
\end{equation}


\vspace{-2pt}\begin{equation}
    \begin{tikzpicture}[baseline={([yshift=-12pt]current bounding box.north)}]

        \node[backtrack] (boxA) at (0, 0) {$x$};
        \node[backtrack] (boxB) [right=1cm of boxA] {$2x$};
        \node[backtrack] (boxC) [right=1cm of boxB] {$2x + 9$};
    
        \node (boxAr) at ([yshift=24pt,xshift=5mm]boxA) { };
        \node (boxBl) at ([yshift=24pt,xshift=-5mm]boxB) { };
        \draw [line width=0.4pt,-{Stealth[length=2mm]}] (boxAr)  --node[backtrackstep, above=3.0pt] {$\times2$} (boxBl);
    
        \node (boxBr) at ([yshift=24pt,xshift=5mm]boxB) { };
        \node (boxCl) at ([yshift=24pt,xshift=-5mm]boxC) { };
        \draw [line width=0.4pt,-{Stealth[length=2mm]}] (boxBr)  --node[backtrackstep, above=3.0pt] {$+9$} (boxCl);
        
    \end{tikzpicture} 
\end{equation}


\vspace{-2pt}\begin{equation}
    \begin{tikzpicture}[baseline={([yshift=-12pt]current bounding box.north)}]

        \node[backtrack] (boxA) at (0, 0) {$x$};
        \node[backtrack] (boxB) [right=1cm of boxA] {$\frac{x}{8}$};
        \node[backtrack] (boxC) [right=1cm of boxB] {$\frac{x}{8} - 9$};
    
        \node (boxAr) at ([yshift=24pt,xshift=5mm]boxA) { };
        \node (boxBl) at ([yshift=24pt,xshift=-5mm]boxB) { };
        \draw [line width=0.4pt,-{Stealth[length=2mm]}] (boxAr)  --node[backtrackstep, above=3.0pt] {$\div8$} (boxBl);
    
        \node (boxBr) at ([yshift=24pt,xshift=5mm]boxB) { };
        \node (boxCl) at ([yshift=24pt,xshift=-5mm]boxC) { };
        \draw [line width=0.4pt,-{Stealth[length=2mm]}] (boxBr)  --node[backtrackstep, above=3.0pt] {$-9$} (boxCl);
        
    \end{tikzpicture} 
\end{equation}


\vspace{-2pt}
    \end{multicols}
\end{document}
